tests/lean/CastSigned.lean
@@ -22,7 +22,7 @@ def test_u8_cast_signed_all_ones : Result Unit := do
   massert (y = (-1)#i8)
 
 /- Unit test for [cast_signed::test_u8_cast_signed_all_ones] -/
-#assert (test_u8_cast_signed_all_ones == ok ())
+#assert ((test_u8_cast_signed_all_ones ).is_ok ())
 
 /-- [cast_signed::test_i8_cast_unsigned_neg_one]:
     Source: 'tests/src/cast_signed.rs', lines 17:0-21:1
@@ -32,7 +32,7 @@ def test_i8_cast_unsigned_neg_one : Result Unit := do
   massert (y = 255#u8)
 
 /- Unit test for [cast_signed::test_i8_cast_unsigned_neg_one] -/
-#assert (test_i8_cast_unsigned_neg_one == ok ())
+#assert ((test_i8_cast_unsigned_neg_one ).is_ok ())
 
 /-- [cast_signed::test_u16_cast_signed_high_bit]:
     Source: 'tests/src/cast_signed.rs', lines 25:0-29:1
@@ -42,7 +42,7 @@ def test_u16_cast_signed_high_bit : Result Unit := do
   massert (y = core.num.I16.MIN)
 
 /- Unit test for [cast_signed::test_u16_cast_signed_high_bit] -/
-#assert (test_u16_cast_signed_high_bit == ok ())
+#assert ((test_u16_cast_signed_high_bit ).is_ok ())
 
 /-- [cast_signed::test_i16_cast_unsigned_neg_one]:
     Source: 'tests/src/cast_signed.rs', lines 33:0-37:1
@@ -52,7 +52,7 @@ def test_i16_cast_unsigned_neg_one : Result Unit := do
   massert (y = core.num.U16.MAX)
 
 /- Unit test for [cast_signed::test_i16_cast_unsigned_neg_one] -/
-#assert (test_i16_cast_unsigned_neg_one == ok ())
+#assert ((test_i16_cast_unsigned_neg_one ).is_ok ())
 
 /-- [cast_signed::test_u32_cast_signed_small]:
     Source: 'tests/src/cast_signed.rs', lines 41:0-45:1
@@ -62,7 +62,7 @@ def test_u32_cast_signed_small : Result Unit := do
   massert (y = 255#i32)
 
 /- Unit test for [cast_signed::test_u32_cast_signed_small] -/
-#assert (test_u32_cast_signed_small == ok ())
+#assert ((test_u32_cast_signed_small ).is_ok ())
 
 /-- [cast_signed::test_u32_cast_signed_all_ones]:
     Source: 'tests/src/cast_signed.rs', lines 49:0-53:1
@@ -72,7 +72,7 @@ def test_u32_cast_signed_all_ones : Result Unit := do
   massert (y = (-1)#i32)
 
 /- Unit test for [cast_signed::test_u32_cast_signed_all_ones] -/
-#assert (test_u32_cast_signed_all_ones == ok ())
+#assert ((test_u32_cast_signed_all_ones ).is_ok ())
 
 /-- [cast_signed::test_u32_cast_signed_high_bit]:
     Source: 'tests/src/cast_signed.rs', lines 57:0-61:1
@@ -82,7 +82,7 @@ def test_u32_cast_signed_high_bit : Result Unit := do
   massert (y = core.num.I32.MIN)
 
 /- Unit test for [cast_signed::test_u32_cast_signed_high_bit] -/
-#assert (test_u32_cast_signed_high_bit == ok ())
+#assert ((test_u32_cast_signed_high_bit ).is_ok ())
 
 /-- [cast_signed::test_i32_cast_unsigned_neg_one]:
     Source: 'tests/src/cast_signed.rs', lines 65:0-69:1
@@ -92,7 +92,7 @@ def test_i32_cast_unsigned_neg_one : Result Unit := do
   massert (y = 4294967295#u32)
 
 /- Unit test for [cast_signed::test_i32_cast_unsigned_neg_one] -/
-#assert (test_i32_cast_unsigned_neg_one == ok ())
+#assert ((test_i32_cast_unsigned_neg_one ).is_ok ())
 
 /-- [cast_signed::test_i32_cast_roundtrip]:
     Source: 'tests/src/cast_signed.rs', lines 73:0-77:1
@@ -103,7 +103,7 @@ def test_i32_cast_roundtrip : Result Unit := do
   massert (y = 3735928559#u32)
 
 /- Unit test for [cast_signed::test_i32_cast_roundtrip] -/
-#assert (test_i32_cast_roundtrip == ok ())
+#assert ((test_i32_cast_roundtrip ).is_ok ())
 
 /-- [cast_signed::test_u64_cast_signed_all_ones]:
     Source: 'tests/src/cast_signed.rs', lines 81:0-85:1
@@ -113,7 +113,7 @@ def test_u64_cast_signed_all_ones : Result Unit := do
   massert (y = (-1)#i64)
 
 /- Unit test for [cast_signed::test_u64_cast_signed_all_ones] -/
-#assert (test_u64_cast_signed_all_ones == ok ())
+#assert ((test_u64_cast_signed_all_ones ).is_ok ())
 
 /-- [cast_signed::test_i64_cast_unsigned_neg_one]:
     Source: 'tests/src/cast_signed.rs', lines 89:0-93:1
@@ -123,7 +123,7 @@ def test_i64_cast_unsigned_neg_one : Result Unit := do
   massert (y = core.num.U64.MAX)
 
 /- Unit test for [cast_signed::test_i64_cast_unsigned_neg_one] -/
-#assert (test_i64_cast_unsigned_neg_one == ok ())
+#assert ((test_i64_cast_unsigned_neg_one ).is_ok ())
 
 /-- [cast_signed::test_u128_cast_signed_all_ones]:
     Source: 'tests/src/cast_signed.rs', lines 97:0-101:1
@@ -133,7 +133,7 @@ def test_u128_cast_signed_all_ones : Result Unit := do
   massert (y = (-1)#i128)
 
 /- Unit test for [cast_signed::test_u128_cast_signed_all_ones] -/
-#assert (test_u128_cast_signed_all_ones == ok ())
+#assert ((test_u128_cast_signed_all_ones ).is_ok ())
 
 /-- [cast_signed::test_i128_cast_unsigned_neg_one]:
     Source: 'tests/src/cast_signed.rs', lines 105:0-109:1
@@ -143,7 +143,7 @@ def test_i128_cast_unsigned_neg_one : Result Unit := do
   massert (y = core.num.U128.MAX)
 
 /- Unit test for [cast_signed::test_i128_cast_unsigned_neg_one] -/
-#assert (test_i128_cast_unsigned_neg_one == ok ())
+#assert ((test_i128_cast_unsigned_neg_one ).is_ok ())
 
 /-- [cast_signed::test_usize_cast_roundtrip]:
     Source: 'tests/src/cast_signed.rs', lines 113:0-117:1
@@ -154,7 +154,7 @@ def test_usize_cast_roundtrip : Result Unit := do
   massert (y = 12345#usize)
 
 /- Unit test for [cast_signed::test_usize_cast_roundtrip] -/
-#assert (test_usize_cast_roundtrip == ok ())
+#assert ((test_usize_cast_roundtrip ).is_ok ())
 
 /-- [cast_signed::test_isize_cast_unsigned_neg_one]:
     Source: 'tests/src/cast_signed.rs', lines 121:0-125:1
@@ -164,6 +164,6 @@ def test_isize_cast_unsigned_neg_one : Result Unit := do
   massert (y = core.num.Usize.MAX)
 
 /- Unit test for [cast_signed::test_isize_cast_unsigned_neg_one] -/
-#assert (test_isize_cast_unsigned_neg_one == ok ())
+#assert ((test_isize_cast_unsigned_neg_one ).is_ok ())
 
 end cast_signed
