tests/lean/IterAdapters.lean
@@ -47,7 +47,7 @@ def test_enumerate_slice : Result Unit := do
   massert b
 
 /- Unit test for [iter_adapters::test_enumerate_slice] -/
-#assert (test_enumerate_slice == ok ())
+#assert ((test_enumerate_slice ).is_ok ())
 
 /-- [iter_adapters::test_enumerate_empty]:
     Source: 'tests/src/iter_adapters.rs', lines 28:0-32:1
@@ -63,7 +63,7 @@ def test_enumerate_empty : Result Unit := do
   massert b
 
 /- Unit test for [iter_adapters::test_enumerate_empty] -/
-#assert (test_enumerate_empty == ok ())
+#assert ((test_enumerate_empty ).is_ok ())
 
 /-- [iter_adapters::test_take_2]:
     Source: 'tests/src/iter_adapters.rs', lines 40:0-46:1
@@ -91,7 +91,7 @@ def test_take_2 : Result Unit := do
   massert b
 
 /- Unit test for [iter_adapters::test_take_2] -/
-#assert (test_take_2 == ok ())
+#assert ((test_take_2 ).is_ok ())
 
 /-- [iter_adapters::test_take_0]:
     Source: 'tests/src/iter_adapters.rs', lines 50:0-54:1
@@ -108,7 +108,7 @@ def test_take_0 : Result Unit := do
   massert b
 
 /- Unit test for [iter_adapters::test_take_0] -/
-#assert (test_take_0 == ok ())
+#assert ((test_take_0 ).is_ok ())
 
 /-- [iter_adapters::test_take_more_than_available]:
     Source: 'tests/src/iter_adapters.rs', lines 58:0-65:1
@@ -139,7 +139,7 @@ def test_take_more_than_available : Result Unit := do
   massert b
 
 /- Unit test for [iter_adapters::test_take_more_than_available] -/
-#assert (test_take_more_than_available == ok ())
+#assert ((test_take_more_than_available ).is_ok ())
 
 /-- [iter_adapters::test_range_u8]: loop body 0:
     Source: 'tests/src/iter_adapters.rs', lines 75:4-77:5
@@ -174,7 +174,7 @@ def test_range_u8 : Result Unit := do
   massert (count = 5#u32)
 
 /- Unit test for [iter_adapters::test_range_u8] -/
-#assert (test_range_u8 == ok ())
+#assert ((test_range_u8 ).is_ok ())
 
 /-- [iter_adapters::test_range_u16]: loop body 0:
     Source: 'tests/src/iter_adapters.rs', lines 85:4-87:5
@@ -211,7 +211,7 @@ def test_range_u16 : Result Unit := do
   massert (count = 4#u32)
 
 /- Unit test for [iter_adapters::test_range_u16] -/
-#assert (test_range_u16 == ok ())
+#assert ((test_range_u16 ).is_ok ())
 
 /-- [iter_adapters::test_range_u32]: loop body 0:
     Source: 'tests/src/iter_adapters.rs', lines 95:4-97:5
@@ -248,7 +248,7 @@ def test_range_u32 : Result Unit := do
   massert (count = 3#u32)
 
 /- Unit test for [iter_adapters::test_range_u32] -/
-#assert (test_range_u32 == ok ())
+#assert ((test_range_u32 ).is_ok ())
 
 /-- [iter_adapters::test_range_u64]: loop body 0:
     Source: 'tests/src/iter_adapters.rs', lines 105:4-107:5
@@ -285,7 +285,7 @@ def test_range_u64 : Result Unit := do
   massert (count = 4#u64)
 
 /- Unit test for [iter_adapters::test_range_u64] -/
-#assert (test_range_u64 == ok ())
+#assert ((test_range_u64 ).is_ok ())
 
 /-- [iter_adapters::test_range_usize]: loop body 0:
     Source: 'tests/src/iter_adapters.rs', lines 115:4-117:5
@@ -324,7 +324,7 @@ def test_range_usize : Result Unit := do
   massert (count = 5#usize)
 
 /- Unit test for [iter_adapters::test_range_usize] -/
-#assert (test_range_usize == ok ())
+#assert ((test_range_usize ).is_ok ())
 
 /-- [iter_adapters::test_range_empty]: loop body 0:
     Source: 'tests/src/iter_adapters.rs', lines 125:4-127:5
@@ -359,7 +359,7 @@ def test_range_empty : Result Unit := do
   massert (count = 0#u32)
 
 /- Unit test for [iter_adapters::test_range_empty] -/
-#assert (test_range_empty == ok ())
+#assert ((test_range_empty ).is_ok ())
 
 /-- [iter_adapters::test_array_into_iter]:
     Source: 'tests/src/iter_adapters.rs', lines 137:0-144:1
@@ -382,7 +382,7 @@ def test_array_into_iter : Result Unit := do
   massert b
 
 /- Unit test for [iter_adapters::test_array_into_iter] -/
-#assert (test_array_into_iter == ok ())
+#assert ((test_array_into_iter ).is_ok ())
 
 /-- [iter_adapters::test_slice_into_iter]:
     Source: 'tests/src/iter_adapters.rs', lines 148:0-157:1
@@ -408,7 +408,7 @@ def test_slice_into_iter : Result Unit := do
   massert b
 
 /- Unit test for [iter_adapters::test_slice_into_iter] -/
-#assert (test_slice_into_iter == ok ())
+#assert ((test_slice_into_iter ).is_ok ())
 
 /-- [iter_adapters::test_enumerate_step_by]:
     Source: 'tests/src/iter_adapters.rs', lines 165:0-172:1
@@ -438,7 +438,7 @@ def test_enumerate_step_by : Result Unit := do
   massert (x1 = 30#u32)
 
 /- Unit test for [iter_adapters::test_enumerate_step_by] -/
-#assert (test_enumerate_step_by == ok ())
+#assert ((test_enumerate_step_by ).is_ok ())
 
 /-- [iter_adapters::test_enumerate_take]:
     Source: 'tests/src/iter_adapters.rs', lines 176:0-184:1
@@ -474,7 +474,7 @@ def test_enumerate_take : Result Unit := do
   massert b
 
 /- Unit test for [iter_adapters::test_enumerate_take] -/
-#assert (test_enumerate_take == ok ())
+#assert ((test_enumerate_take ).is_ok ())
 
 /-- [iter_adapters::test_take_exhausted_then_next]:
     Source: 'tests/src/iter_adapters.rs', lines 188:0-197:1
@@ -500,7 +500,7 @@ def test_take_exhausted_then_next : Result Unit := do
   massert b1
 
 /- Unit test for [iter_adapters::test_take_exhausted_then_next] -/
-#assert (test_take_exhausted_then_next == ok ())
+#assert ((test_take_exhausted_then_next ).is_ok ())
 
 /-- [iter_adapters::test_range_single_element]:
     Source: 'tests/src/iter_adapters.rs', lines 206:0-210:1
@@ -516,7 +516,7 @@ def test_range_single_element : Result Unit := do
   massert b
 
 /- Unit test for [iter_adapters::test_range_single_element] -/
-#assert (test_range_single_element == ok ())
+#assert ((test_range_single_element ).is_ok ())
 
 /-- [iter_adapters::test_range_u8_near_max]:
     Source: 'tests/src/iter_adapters.rs', lines 214:0-218:1
@@ -532,7 +532,7 @@ def test_range_u8_near_max : Result Unit := do
   massert b
 
 /- Unit test for [iter_adapters::test_range_u8_near_max] -/
-#assert (test_range_u8_near_max == ok ())
+#assert ((test_range_u8_near_max ).is_ok ())
 
 /-- [iter_adapters::test_range_u8_start_gt_end]:
     Source: 'tests/src/iter_adapters.rs', lines 222:0-225:1
@@ -545,7 +545,7 @@ def test_range_u8_start_gt_end : Result Unit := do
   massert b
 
 /- Unit test for [iter_adapters::test_range_u8_start_gt_end] -/
-#assert (test_range_u8_start_gt_end == ok ())
+#assert ((test_range_u8_start_gt_end ).is_ok ())
 
 /-- [iter_adapters::test_range_u8_start_eq_end]:
     Source: 'tests/src/iter_adapters.rs', lines 229:0-232:1
@@ -558,7 +558,7 @@ def test_range_u8_start_eq_end : Result Unit := do
   massert b
 
 /- Unit test for [iter_adapters::test_range_u8_start_eq_end] -/
-#assert (test_range_u8_start_eq_end == ok ())
+#assert ((test_range_u8_start_eq_end ).is_ok ())
 
 /-- [iter_adapters::test_range_u16_boundary]:
     Source: 'tests/src/iter_adapters.rs', lines 236:0-242:1
@@ -583,7 +583,7 @@ def test_range_u16_boundary : Result Unit := do
   massert b
 
 /- Unit test for [iter_adapters::test_range_u16_boundary] -/
-#assert (test_range_u16_boundary == ok ())
+#assert ((test_range_u16_boundary ).is_ok ())
 
 /-- [iter_adapters::test_range_u32_boundary]:
     Source: 'tests/src/iter_adapters.rs', lines 246:0-251:1
@@ -604,7 +604,7 @@ def test_range_u32_boundary : Result Unit := do
   massert b
 
 /- Unit test for [iter_adapters::test_range_u32_boundary] -/
-#assert (test_range_u32_boundary == ok ())
+#assert ((test_range_u32_boundary ).is_ok ())
 
 /-- [iter_adapters::test_range_u64_boundary]:
     Source: 'tests/src/iter_adapters.rs', lines 255:0-261:1
@@ -629,7 +629,7 @@ def test_range_u64_boundary : Result Unit := do
   massert b
 
 /- Unit test for [iter_adapters::test_range_u64_boundary] -/
-#assert (test_range_u64_boundary == ok ())
+#assert ((test_range_u64_boundary ).is_ok ())
 
 /-- [iter_adapters::test_range_usize_start_gt_end]:
     Source: 'tests/src/iter_adapters.rs', lines 265:0-268:1
@@ -642,7 +642,7 @@ def test_range_usize_start_gt_end : Result Unit := do
   massert b
 
 /- Unit test for [iter_adapters::test_range_usize_start_gt_end] -/
-#assert (test_range_usize_start_gt_end == ok ())
+#assert ((test_range_usize_start_gt_end ).is_ok ())
 
 /-- [iter_adapters::test_step_by_larger_than_range]:
     Source: 'tests/src/iter_adapters.rs', lines 272:0-276:1
@@ -663,7 +663,7 @@ def test_step_by_larger_than_range : Result Unit := do
   massert b
 
 /- Unit test for [iter_adapters::test_step_by_larger_than_range] -/
-#assert (test_step_by_larger_than_range == ok ())
+#assert ((test_step_by_larger_than_range ).is_ok ())
 
 /-- [iter_adapters::test_step_by_exact_range]:
     Source: 'tests/src/iter_adapters.rs', lines 280:0-284:1
@@ -684,7 +684,7 @@ def test_step_by_exact_range : Result Unit := do
   massert b
 
 /- Unit test for [iter_adapters::test_step_by_exact_range] -/
-#assert (test_step_by_exact_range == ok ())
+#assert ((test_step_by_exact_range ).is_ok ())
 
 /-- [iter_adapters::test_step_by_one]:
     Source: 'tests/src/iter_adapters.rs', lines 288:0-295:1
@@ -720,7 +720,7 @@ def test_step_by_one : Result Unit := do
   massert b
 
 /- Unit test for [iter_adapters::test_step_by_one] -/
-#assert (test_step_by_one == ok ())
+#assert ((test_step_by_one ).is_ok ())
 
 /-- [iter_adapters::test_step_by_empty]:
     Source: 'tests/src/iter_adapters.rs', lines 299:0-302:1
@@ -736,7 +736,7 @@ def test_step_by_empty : Result Unit := do
   massert b
 
 /- Unit test for [iter_adapters::test_step_by_empty] -/
-#assert (test_step_by_empty == ok ())
+#assert ((test_step_by_empty ).is_ok ())
 
 /-- [iter_adapters::test_step_by_odd_range]:
     Source: 'tests/src/iter_adapters.rs', lines 306:0-312:1
@@ -767,7 +767,7 @@ def test_step_by_odd_range : Result Unit := do
   massert b
 
 /- Unit test for [iter_adapters::test_step_by_odd_range] -/
-#assert (test_step_by_odd_range == ok ())
+#assert ((test_step_by_odd_range ).is_ok ())
 
 /-- [iter_adapters::test_step_by_u8_near_max]:
     Source: 'tests/src/iter_adapters.rs', lines 316:0-322:1
@@ -798,7 +798,7 @@ def test_step_by_u8_near_max : Result Unit := do
   massert b
 
 /- Unit test for [iter_adapters::test_step_by_u8_near_max] -/
-#assert (test_step_by_u8_near_max == ok ())
+#assert ((test_step_by_u8_near_max ).is_ok ())
 
 /-- [iter_adapters::test_range_inclusive_basic]:
     Source: 'tests/src/iter_adapters.rs', lines 330:0-336:1
@@ -827,7 +827,7 @@ def test_range_inclusive_basic : Result Unit := do
   massert b
 
 /- Unit test for [iter_adapters::test_range_inclusive_basic] -/
-#assert (test_range_inclusive_basic == ok ())
+#assert ((test_range_inclusive_basic ).is_ok ())
 
 /-- [iter_adapters::test_range_inclusive_singleton]:
     Source: 'tests/src/iter_adapters.rs', lines 340:0-344:1
@@ -846,7 +846,7 @@ def test_range_inclusive_singleton : Result Unit := do
   massert b
 
 /- Unit test for [iter_adapters::test_range_inclusive_singleton] -/
-#assert (test_range_inclusive_singleton == ok ())
+#assert ((test_range_inclusive_singleton ).is_ok ())
 
 /-- [iter_adapters::test_range_inclusive_empty]:
     Source: 'tests/src/iter_adapters.rs', lines 348:0-351:1
@@ -860,6 +860,6 @@ def test_range_inclusive_empty : Result Unit := do
   massert b
 
 /- Unit test for [iter_adapters::test_range_inclusive_empty] -/
-#assert (test_range_inclusive_empty == ok ())
+#assert ((test_range_inclusive_empty ).is_ok ())
 
 end iter_adapters
